Made concurrency pointer-size-agnostic.

concurrency/lksize.v
@@ -3,5 +3,11 @@ Require Import compcert.common.Memdata.
 Require Import Coq.ZArith.ZArith.
 
 (* LKSIZE should match sizeof(semax_conc.tlock).  *)
-Definition LKSIZE:= 8%Z.
+Definition LKSIZE:= (2 * size_chunk Mptr)%Z.
 Definition LKSIZE_nat:= Z.to_nat LKSIZE.
+
+Lemma LKSIZE_pos : (0 < LKSIZE)%Z.
+Proof.
+  unfold LKSIZE.
+  pose proof (size_chunk_pos Mptr); omega.
+Qed.
