concurrency/dry_machine.v
@@ -317,24 +317,24 @@ Module Concur.
              (** install the thread's permissions on lock locations*)
              (Hrestrict_pmap0: restrPermMap (Hcompat tid0 cnt0).2 = m0)
              (** To acquire the lock the thread must have [Readable] permission on it*)
-             (Haccess: Mem.range_perm m0 b (Int.intval ofs) ((Int.intval ofs) + LKSIZE) Cur Readable)
+             (Haccess: Mem.range_perm m0 b (Ptrofs.intval ofs) ((Ptrofs.intval ofs) + LKSIZE) Cur Readable)
              (** check if the lock is free*)
-             (Hload: Mem.load Mint32 m0 b (Int.intval ofs) = Some (Vint Int.one))
+             (Hload: Mem.load Mint32 m0 b (Ptrofs.intval ofs) = Some (Vint Int.one))
              (** set the permissions on the lock location equal to the max permissions on the memory*)
              (Hset_perm: setPermBlock (Some Writable)
-                                       b (Int.intval ofs) ((getThreadR cnt0).2) LKSIZE_nat = pmap_tid')
+                                       b (Ptrofs.intval ofs) ((getThreadR cnt0).2) LKSIZE_nat = pmap_tid')
              (Hlt': permMapLt pmap_tid' (getMaxPerm m))
              (Hrestrict_pmap: restrPermMap Hlt' = m1)
              (** acquire the lock*)
-             (Hstore: Mem.store Mint32 m1 b (Int.intval ofs) (Vint Int.zero) = Some m')
-             (HisLock: lockRes tp (b, Int.intval ofs) = Some pmap)
+             (Hstore: Mem.store Mint32 m1 b (Ptrofs.intval ofs) (Vint Int.zero) = Some m')
+             (HisLock: lockRes tp (b, Ptrofs.intval ofs) = Some pmap)
              (Hangel1: permMapJoin pmap.1 (getThreadR cnt0).1 newThreadPerm.1)
              (Hangel2: permMapJoin pmap.2 (getThreadR cnt0).2 newThreadPerm.2)
              (Htp': tp' = updThread cnt0 (Kresume c Vundef) newThreadPerm)
              (** acquiring the lock leaves empty permissions at the resource pool*)
-             (Htp'': tp'' = updLockSet tp' (b, Int.intval ofs) (empty_map, empty_map)),
+             (Htp'': tp'' = updLockSet tp' (b, Ptrofs.intval ofs) (empty_map, empty_map)),
              ext_step genv cnt0 Hcompat tp'' m'
-                      (acquire (b, Int.intval ofs)
+                      (acquire (b, Ptrofs.intval ofs)
                                (Some virtueThread))
 
      | step_release :
@@ -361,16 +361,16 @@ Module Concur.
              (** install the thread's permissions on lock locations *)
              (Hrestrict_pmap0: restrPermMap (Hcompat tid0 cnt0).2 = m0)
              (** To acquire the lock the thread must have [Readable] permission on it*)
-             (Haccess: Mem.range_perm m0 b (Int.intval ofs) ((Int.intval ofs) + LKSIZE) Cur Readable)
-             (Hload: Mem.load Mint32 m0 b (Int.intval ofs) = Some (Vint Int.zero))
+             (Haccess: Mem.range_perm m0 b (Ptrofs.intval ofs) ((Ptrofs.intval ofs) + LKSIZE) Cur Readable)
+             (Hload: Mem.load Mint32 m0 b (Ptrofs.intval ofs) = Some (Vint Int.zero))
              (** set the permissions on the lock location equal to the max permissions on the memory*)
              (Hset_perm: setPermBlock (Some Writable)
-                                      b (Int.intval ofs) ((getThreadR cnt0).2) LKSIZE_nat = pmap_tid')
+                                      b (Ptrofs.intval ofs) ((getThreadR cnt0).2) LKSIZE_nat = pmap_tid')
              (Hlt': permMapLt pmap_tid' (getMaxPerm m))
              (Hrestrict_pmap: restrPermMap Hlt' = m1)
              (** release the lock *)
-             (Hstore: Mem.store Mint32 m1 b (Int.intval ofs) (Vint Int.one) = Some m')
-             (HisLock: lockRes tp (b, Int.intval ofs) = Some rmap)
+             (Hstore: Mem.store Mint32 m1 b (Ptrofs.intval ofs) (Vint Int.one) = Some m')
+             (HisLock: lockRes tp (b, Ptrofs.intval ofs) = Some rmap)
              (** And the lock is taken*)
              (Hrmap: forall b ofs, rmap.1 !! b ofs = None /\ rmap.2 !! b ofs = None)
              (Hangel1: permMapJoin newThreadPerm.1 virtueLP.1 (getThreadR cnt0).1)
@@ -378,9 +378,9 @@ Module Concur.
              (Htp': tp' = updThread cnt0 (Kresume c Vundef)
                                     (computeMap (getThreadR cnt0).1 virtueThread.1,
                                      computeMap (getThreadR cnt0).2 virtueThread.2))
-             (Htp'': tp'' = updLockSet tp' (b, Int.intval ofs) virtueLP),
+             (Htp'': tp'' = updLockSet tp' (b, Ptrofs.intval ofs) virtueLP),
              ext_step genv cnt0 Hcompat tp'' m'
-                      (release (b, Int.intval ofs)
+                      (release (b, Ptrofs.intval ofs)
                                (Some virtueLP))
      | step_create :
          forall (tp_upd tp':thread_pool) c b ofs arg virtue1 virtue2
@@ -409,7 +409,7 @@ Module Concur.
            (Htp_upd: tp_upd = updThread cnt0 (Kresume c Vundef) threadPerm')
            (Htp': tp' = addThread tp_upd (Vptr b ofs) arg newThreadPerm),
              ext_step genv cnt0 Hcompat tp' m
-                      (spawn (b, Int.intval ofs)
+                      (spawn (b, Ptrofs.intval ofs)
                              (Some (getThreadR cnt0, virtue1)) (Some virtue2))
 
 
@@ -423,29 +423,29 @@ Module Concur.
              (** install the thread's data permissions*)
              (Hrestrict_pmap: restrPermMap (Hcompat tid0 cnt0).1 = m1)
              (** To create the lock the thread must have [Writable] permission on it*)
-             (Hfreeable: Mem.range_perm m1 b (Int.intval ofs) ((Int.intval ofs) + LKSIZE) Cur Writable)
+             (Hfreeable: Mem.range_perm m1 b (Ptrofs.intval ofs) ((Ptrofs.intval ofs) + LKSIZE) Cur Writable)
              (** lock is created in acquired state*)
-             (Hstore: Mem.store Mint32 m1 b (Int.intval ofs) (Vint Int.zero) = Some m')
+             (Hstore: Mem.store Mint32 m1 b (Ptrofs.intval ofs) (Vint Int.zero) = Some m')
              (** The thread's data permissions are set to Nonempty*)
              (Hdata_perm: setPermBlock
                             (Some Nonempty)
                             b
-                            (Int.intval ofs)
+                            (Ptrofs.intval ofs)
                             pmap_tid.1
                             LKSIZE_nat = pmap_tid'.1)
              (** thread lock permission is increased *)
              (Hlock_perm: setPermBlock
                             (Some Writable)
                             b
-                            (Int.intval ofs)
+                            (Ptrofs.intval ofs)
                             pmap_tid.2
                             LKSIZE_nat = pmap_tid'.2)
-             (** Require that [(b, Int.intval ofs)] was not a lock*)
-             (HlockRes: lockRes tp (b, Int.intval ofs) = None)
+             (** Require that [(b, Ptrofs.intval ofs)] was not a lock*)
+             (HlockRes: lockRes tp (b, Ptrofs.intval ofs) = None)
              (Htp': tp' = updThread cnt0 (Kresume c Vundef) pmap_tid')
              (** the lock has no resources initially *)
-             (Htp'': tp'' = updLockSet tp' (b, Int.intval ofs) (empty_map, empty_map)),
-             ext_step genv cnt0 Hcompat tp'' m' (mklock (b, Int.intval ofs))
+             (Htp'': tp'' = updLockSet tp' (b, Ptrofs.intval ofs) (empty_map, empty_map)),
+             ext_step genv cnt0 Hcompat tp'' m' (mklock (b, Ptrofs.intval ofs))
 
      | step_freelock :
          forall  (tp' tp'': thread_pool) c b ofs pmap_tid' m1 pdata rmap
@@ -459,18 +459,18 @@ Module Concur.
            (Hcode: getThreadC cnt0 = Kblocked c)
            (Hat_external: at_external Sem genv c m = Some (FREE_LOCK, Vptr b ofs::nil))
            (** If this address is a lock*)
-           (His_lock: lockRes tp (b, (Int.intval ofs)) = Some rmap)
+           (His_lock: lockRes tp (b, (Ptrofs.intval ofs)) = Some rmap)
            (** And the lock is taken *)
            (Hrmap: forall b ofs, rmap.1 !! b ofs = None /\ rmap.2 !! b ofs = None)
            (** Install the thread's lock permissions*)
            (Hrestrict_pmap: restrPermMap (Hcompat tid0 cnt0).2 = m1)
            (** To free the lock the thread must have at least Writable on it*)
-           (Hfreeable: Mem.range_perm m1 b (Int.intval ofs) ((Int.intval ofs) + LKSIZE) Cur Writable)
+           (Hfreeable: Mem.range_perm m1 b (Ptrofs.intval ofs) ((Ptrofs.intval ofs) + LKSIZE) Cur Writable)
            (** lock permissions of the thread are dropped to empty *)
            (Hlock_perm: setPermBlock
                           None
                           b
-                          (Int.intval ofs)
+                          (Ptrofs.intval ofs)
                           pmap_tid.2
                           LKSIZE_nat = pmap_tid'.2)
            (** data permissions are computed in a non-deterministic way *)
@@ -482,12 +482,12 @@ Module Concur.
            (Hdata_perm: setPermBlock_var (*=setPermBlockfunc*)
                           pdata
                           b
-                          (Int.intval ofs)
+                          (Ptrofs.intval ofs)
                           pmap_tid.1
                           LKSIZE_nat = pmap_tid'.1)
            (Htp': tp' = updThread cnt0 (Kresume c Vundef) pmap_tid')
-           (Htp'': tp'' = remLockSet tp' (b, Int.intval ofs)),
-           ext_step genv cnt0 Hcompat  tp'' m (freelock (b, Int.intval ofs))
+           (Htp'': tp'' = remLockSet tp' (b, Ptrofs.intval ofs)),
+           ext_step genv cnt0 Hcompat  tp'' m (freelock (b, Ptrofs.intval ofs))
      | step_acqfail :
          forall  c b ofs m1
            (Hinv : invariant tp)
@@ -496,10 +496,10 @@ Module Concur.
            (** Install the thread's lock permissions*)
            (Hrestrict_pmap: restrPermMap (Hcompat tid0 cnt0).2 = m1)
            (** To acquire the lock the thread must have [Readable] permission on it*)
-           (Haccess: Mem.range_perm m1 b (Int.intval ofs) ((Int.intval ofs) + LKSIZE) Cur Readable)
+           (Haccess: Mem.range_perm m1 b (Ptrofs.intval ofs) ((Ptrofs.intval ofs) + LKSIZE) Cur Readable)
            (** Lock is already acquired.*)
-           (Hload: Mem.load Mint32 m1 b (Int.intval ofs) = Some (Vint Int.zero)),
-           ext_step genv cnt0 Hcompat tp m (failacq (b, Int.intval ofs)).
+           (Hload: Mem.load Mint32 m1 b (Ptrofs.intval ofs) = Some (Vint Int.zero)),
+           ext_step genv cnt0 Hcompat tp m (failacq (b, Ptrofs.intval ofs)).
 
      Definition threadStep (genv : G): forall {tid0 ms m},
          containsThread ms tid0 -> mem_compatible ms m ->
