concurrency/threadPool.v
@@ -529,17 +529,14 @@ Import Coqlib.
     apply SetoidList.InA_cons in H1.
     destruct H1.
     hnf in H0. destruct a; simpl in H0. destruct H0; subst a l0.
-    simpl. unfold permissions.setPerm. rewrite !PMap.gss.
-    repeat match goal with |- context [is_left ?A] => destruct A; simpl; auto end.
-    omega.
+    simpl. rewrite setPermBlock_lookup.
+    if_tac; auto.
+    simpl in H0; tauto.
     apply IHel in H0; clear IHel.
     simpl.
     unfold f at 1. destruct a. destruct a.
-    unfold permissions.setPermBlock. simpl.
-    unfold permissions.setPerm. rewrite !PMap.gss.
-    destruct (peq b0 b). subst b0. rewrite !PMap.gss.
-    repeat match goal with |- context [is_left ?A] => destruct A; simpl; auto end.
-    rewrite !PMap.gso; auto.
+    rewrite setPermBlock_lookup.
+    if_tac; auto.
   Qed.
 
   Lemma lockSet_spec_1: forall js b ofs,
@@ -549,7 +546,10 @@ Import Coqlib.
     intros.
     eapply lockSet_spec_2; eauto.
     unfold Intv.In.
-    simpl. omega.
+    simpl.
+    unfold LKSIZE_nat.
+    pose proof LKSIZE_pos.
+    rewrite Z2Nat.id; omega.
   Qed.
 
 Open Scope nat_scope.
@@ -1008,7 +1008,7 @@ Lemma lockRes_range_dec: forall tp b ofs,
     { (exists z, z <= ofs < z+LKSIZE /\ lockRes tp (b,z) )%Z  } + {(forall z, z <= ofs < z+LKSIZE -> lockRes tp (b,z) = None)%Z }.
 Proof.
   intros tp b ofs.
-  assert (H : (0 <= LKSIZE)%Z). unfold LKSIZE; omega.
+  assert (H : (0 <= LKSIZE)%Z). pose proof LKSIZE_pos; omega.
   destruct (@RiemannInt_SF.IZN_var _ H) as (n, ->).
   induction n.
   - right. simpl. intros. omega.
@@ -1051,17 +1051,10 @@ Proof.
   simpl. rewrite PMap.gi. auto.
   change ((f a (fold_right f init al)) !! b ofs = None).
   unfold f at 1. destruct a as [[? ?] ?].
-  simpl.
-  destruct (peq b0 b).
-   2: unfold permissions.setPerm; rewrite !PMap.gso; auto.
-  subst b0; rewrite !PMap.gss.
-  cut (~ (z <= ofs < z+LKSIZE))%Z.
-  unfold LKSIZE.
-   intro.
-  repeat match goal with |- context [is_left ?A] => destruct A; [ omega | simpl ] end.
-  apply IHal. intros. apply H7. right; auto.
-  intro.
-  apply H' in H. apply H; clear H.
+  rewrite setPermBlock_lookup.
+  if_tac; auto.
+  destruct H; subst.
+  exfalso; eapply H'; eauto.
   specialize (H7 (b,z) l). spec H7; [left; reflexivity |].
   exists l; auto.
 Qed.
@@ -1089,7 +1082,7 @@ Qed.
    * hnf in H.
      destruct (lockRes ds (b,z)) eqn:?; inv H1.
      + destruct (lockRes ds (b,ofs)) eqn:?; inv H4.
-       assert (z <= ofs < z+16 \/ ofs <= z <= ofs+16)%Z by omega.
+       assert (z <= ofs < z+2 * size_chunk AST.Mptr \/ ofs <= z <= ofs+2 * size_chunk AST.Mptr)%Z by omega.
          destruct H1.
          - specialize (H b z). rewrite Heqo in H. unfold LKSIZE in H.
               specialize (H ofs). spec H; [omega|]. congruence.
@@ -1139,9 +1132,9 @@ Qed.
     destruct (lockRes_range_dec ds b ofs').
     - destruct e as [z [ineq HH]]. unfold LKSIZE in ineq.
       assert (ofs <> z).
-      { intros AA. inversion AA.
-        apply H0. hnf. unfold LKSIZE.
-        simpl; omega. }
+      { intro; subst.
+        apply H0. hnf. simpl. unfold LKSIZE.
+        omega. }
       erewrite lockSet_spec_2.
       erewrite lockSet_spec_2; auto.
       + hnf; simpl; eauto.
@@ -1755,7 +1748,9 @@ Qed.
       (Maps.PMap.get b (lockSet tp)) ofs'.
   Proof.
     intros.
-    apply gsoLockSet_12. intros [? ?]. unfold LKSIZE in *; simpl in *; omega.
+    apply gsoLockSet_12. intros [? ?].
+    pose proof LKSIZE_pos.
+    unfold LKSIZE_nat in Hofs; rewrite Z2Nat.id in Hofs; omega.
   Qed.
 
   Lemma gsoLockSet_2 :
@@ -2310,17 +2305,13 @@ Import Coqlib.
     apply SetoidList.InA_cons in H1.
     destruct H1.
     hnf in H0. destruct a; simpl in H0. destruct H0; subst.
-    simpl. unfold permissions.setPerm. rewrite !PMap.gss.
-    repeat match goal with |- context [is_left ?A] => destruct A; simpl; auto end.
-    omega.
+    simpl. rewrite setPermBlock_lookup. if_tac; auto.
+    contradiction H0; split; auto; omega.
     apply IHel in H0; clear IHel.
     simpl.
     unfold f at 1. destruct a. destruct a.
-    unfold permissions.setPermBlock. simpl.
-    unfold permissions.setPerm. rewrite !PMap.gss.
-    destruct (peq b0 b). subst b0. rewrite !PMap.gss.
-    repeat match goal with |- context [is_left ?A] => destruct A; simpl; auto end.
-    rewrite !PMap.gso; auto.
+    rewrite setPermBlock_lookup.
+    if_tac; auto.
   Qed.
 
   Lemma lockSet_spec_1: forall js b ofs,
@@ -2330,7 +2321,10 @@ Import Coqlib.
     intros.
     eapply lockSet_spec_2; eauto.
     unfold Intv.In.
-    simpl. omega.
+    simpl.
+    unfold LKSIZE_nat.
+    pose proof LKSIZE_pos.
+    rewrite Z2Nat.id; omega.
   Qed.
 
 Open Scope nat_scope.
@@ -2789,7 +2783,7 @@ Lemma lockRes_range_dec: forall tp b ofs,
     { (exists z, z <= ofs < z+LKSIZE /\ lockRes tp (b,z) )%Z  } + {(forall z, z <= ofs < z+LKSIZE -> lockRes tp (b,z) = None)%Z }.
 Proof.
   intros tp b ofs.
-  assert (H : (0 <= LKSIZE)%Z). unfold LKSIZE; omega.
+  assert (H : (0 <= LKSIZE)%Z). pose proof LKSIZE_pos; omega.
   destruct (@RiemannInt_SF.IZN_var _ H) as (n, ->).
   induction n.
   - right. simpl. intros. omega.
@@ -2832,17 +2826,10 @@ Proof.
   simpl. rewrite PMap.gi. auto.
   change ((f a (fold_right f init al)) !! b ofs = None).
   unfold f at 1. destruct a as [[? ?] ?].
-  simpl.
-  destruct (peq b0 b).
-   2: unfold permissions.setPerm; rewrite !PMap.gso; auto.
-  subst b0; rewrite !PMap.gss.
-  cut (~ (z <= ofs < z+LKSIZE))%Z.
-  unfold LKSIZE.
-   intro.
-  repeat match goal with |- context [is_left ?A] => destruct A; [ omega | simpl ] end.
-  apply IHal. intros. apply H7. right; auto.
-  intro.
-  apply H' in H. apply H; clear H.
+  rewrite setPermBlock_lookup.
+  if_tac; auto.
+  destruct H; subst.
+  exfalso; eapply H'; eauto.
   specialize (H7 (b,z) r). spec H7; [left; reflexivity |].
   exists r; auto.
 Qed.
@@ -2870,7 +2857,7 @@ Qed.
    * hnf in H.
      destruct (lockRes ds (b,z)) eqn:?; inv H1.
      + destruct (lockRes ds (b,ofs)) eqn:?; inv H4.
-       assert (z <= ofs < z+16 \/ ofs <= z <= ofs+16)%Z by omega.
+       assert (z <= ofs < z+2 * size_chunk AST.Mptr \/ ofs <= z <= ofs+2 * size_chunk AST.Mptr)%Z by omega.
          destruct H1.
          - specialize (H b z). rewrite Heqo in H. unfold LKSIZE in H.
               specialize (H ofs). spec H; [omega|]. congruence.
@@ -2921,8 +2908,8 @@ Qed.
     - destruct e as [z [ineq HH]]. unfold LKSIZE in ineq.
       assert (ofs <> z).
       { intros AA. inversion AA.
-        apply H0. hnf. unfold LKSIZE.
-        simpl; omega. }
+        apply H0. hnf. simpl.
+        unfold LKSIZE; omega. }
       erewrite lockSet_spec_2.
       erewrite lockSet_spec_2; auto.
       + hnf; simpl; eauto.
@@ -3536,7 +3523,9 @@ Qed.
       (Maps.PMap.get b (lockSet tp)) ofs'.
   Proof.
     intros.
-    apply gsoLockSet_12. intros [? ?]. unfold LKSIZE in *; simpl in *; omega.
+    apply gsoLockSet_12. intros [? ?].
+    pose proof LKSIZE_pos.
+    unfold LKSIZE_nat in Hofs; rewrite Z2Nat.id in Hofs; omega.
   Qed.
 
   Lemma gsoLockSet_2 :
