Makefile
@@ -118,7 +118,7 @@ CONCUR_FILES= \
   concurrent_machine.v disjointness.v dry_context.v dry_machine.v \
   dry_machine_lemmas.v dry_machine_step_lemmas.v \
   Clight_bounds.v enums_equality.v\
-  ClightSemantincsForMachines.v Clight_coreSemantincsForMachines.v \
+  ClightSemantincsForMachines.v ClightCoreSemantincsForMachines.v \
   JuicyMachineModule.v DryMachineSource.v \
   erased_machine.v erasure_proof.v erasure_safety.v erasure_signature.v \
   fineConc_safe.v inj_lemmas.v join_sm.v juicy_machine.v \
